SSA/Projects/LLVMAndRiscv.lean
@@ -31,33 +31,22 @@ see: section (UnrealizedConversionCastOp)
 https://mlir.llvm.org/docs/Dialects/Builtin/#builtinunrealized_conversion_cast-unrealizedconversioncastop
  -/
 
-/-- Defining an instance for LLVM.Ty from InstCombine.Ty instance.-/
-instance : DecidableEq LLVM.Ty :=
-  fun a b => by
-    simp only [LLVM] at a b
-    exact (inferInstanceAs (DecidableEq (InstCombine.MTy 0)) a b)
-
-/-- Defining an instance for LLVM.Op from InstCombine.Op instance. -/
-instance : DecidableEq LLVM.Op :=
-  fun a b => by
-    simp only [LLVM] at a b
-    exact (inferInstanceAs (DecidableEq (InstCombine.MOp 0)) a b)
-
 inductive Ty where
-  | llvm : (LLVM.Ty) -> Ty
-  | riscv : (Dialect.Ty RISCV64.RV64) -> Ty
+  | llvm : LLVM.Ty -> Ty
+  | riscv : RISCV64.RV64.Ty -> Ty
   deriving DecidableEq, Repr
 
 inductive Op where
-  | llvm : (Dialect.Op LLVM) -> Op
-  | riscv : (Dialect.Op RISCV64.RV64) -> Op
+  | llvm : LLVM.Op -> Op
+  | riscv : RISCV64.RV64.Op -> Op
   | builtin.unrealized_conversion_cast.riscvToLLVM : Op
   | builtin.unrealized_conversion_cast.LLVMToriscv : Op
   deriving DecidableEq, Repr
 
 /-- Semantics of an unrealized conversion cast from RISC-V 64 to LLVM.
 We wrap `BitVec 64`in `Option (BitVec 64)` -/
-def builtin.unrealized_conversion_cast.riscvToLLVM (toCast : BitVec 64 ) : Option (BitVec 64 ) := some toCast
+def builtin.unrealized_conversion_cast.riscvToLLVM (toCast : BitVec 64) : PoisonOr (BitVec 64) :=
+  .value toCast
 
 /--
 Semantics of an unrealized conversion cast from LLVM to RISC-V.
@@ -65,14 +54,15 @@ This cast attempts to lower an `(Option (BitVec 64))` to a concrete `(BitVec 64)
 If the value is `some`, we extract the underlying `BitVec`.
 If it is `none` (e.g., an LLVM poison value), we default to the zero `BitVec`.
 -/
-def builtin.unrealized_conversion_cast.LLVMToriscv (toCast : Option (BitVec 64)) : BitVec 64 := toCast.getD 0#64
+def builtin.unrealized_conversion_cast.LLVMToriscv (toCast : PoisonOr (BitVec 64)) : BitVec 64 :=
+  toCast.toOption.getD 0#64
 
 @[simp]
 abbrev LLVMPlusRiscV : Dialect where
   Op := Op
   Ty := Ty
 
-instance : TyDenote (Dialect.Ty LLVMPlusRiscV) where
+instance : TyDenote LLVMPlusRiscV.Ty where
   toType := fun
     | .llvm llvmTy => TyDenote.toType llvmTy
     | .riscv riscvTy => TyDenote.toType riscvTy
@@ -87,32 +77,37 @@ instance LLVMPlusRiscVSignature : DialectSignature LLVMPlusRiscV where
   | .builtin.unrealized_conversion_cast.LLVMToriscv =>
       {sig := [Ty.llvm (.bitvec 64)], outTy := (Ty.riscv .bv), regSig := []}
 
-instance : ToString (Dialect.Ty LLVMPlusRiscV)  where
+instance : ToString LLVMPlusRiscV.Ty  where
   toString t := repr t |>.pretty
 
 @[simp_denote]
-def llvmArgsFromHybrid : {tys : List LLVM.Ty} → HVector TyDenote.toType (tys.map LLVMRiscV.Ty.llvm) → HVector TyDenote.toType tys
+def llvmArgsFromHybrid : {tys : List LLVM.Ty} →
+  HVector TyDenote.toType (tys.map LLVMRiscV.Ty.llvm) → HVector TyDenote.toType tys
   | [], .nil => .nil
   | _ :: _, .cons x xs => .cons x (llvmArgsFromHybrid xs)
 
 @[simp_denote]
-def riscvArgsFromHybrid : {tys : List RISCV64.RV64.Ty} → HVector TyDenote.toType (tys.map LLVMRiscV.Ty.riscv) → HVector TyDenote.toType tys
+def riscvArgsFromHybrid : {tys : List RISCV64.RV64.Ty} →
+  HVector TyDenote.toType (tys.map LLVMRiscV.Ty.riscv) → HVector TyDenote.toType tys
   | [], .nil => .nil
   | _ :: _, .cons x xs => .cons x (riscvArgsFromHybrid xs)
 
 @[simp, reducible]
 instance : DialectDenote (LLVMPlusRiscV) where
   denote
-  | .llvm (llvmOp), args , .nil => DialectDenote.denote llvmOp (llvmArgsFromHybrid args) .nil
-  | .riscv (riscvOp), args , .nil => DialectDenote.denote riscvOp (riscvArgsFromHybrid args) .nil
+  | .llvm (llvmOp), args, .nil =>
+      DialectDenote.denote llvmOp (llvmArgsFromHybrid args) .nil
+  | .riscv (riscvOp), args, .nil =>
+      DialectDenote.denote riscvOp (riscvArgsFromHybrid args) .nil
   | .builtin.unrealized_conversion_cast.riscvToLLVM, elemToCast, _ =>
-    let toCast : (BitVec 64) := (elemToCast.getN 0 (by simp [DialectSignature.sig, signature])) -- adapting to the newly introduced PoisonOr wrapper.
-    let casted : Option (BitVec 64) := builtin.unrealized_conversion_cast.riscvToLLVM toCast
-    PoisonOr.ofOption casted
+    let toCast : BitVec 64 :=
+      elemToCast.getN 0 (by simp [DialectSignature.sig, signature]) -- adapting to the newly introduced PoisonOr wrapper.
+    builtin.unrealized_conversion_cast.riscvToLLVM toCast
   | .builtin.unrealized_conversion_cast.LLVMToriscv,
     (elemToCast : HVector TyDenote.toType [Ty.llvm (.bitvec 64)]), _ =>
-    let toCast : PoisonOr (BitVec 64) := (elemToCast.getN 0 (by simp [DialectSignature.sig, signature]))
-    builtin.unrealized_conversion_cast.LLVMToriscv toCast.toOption
+    let toCast : PoisonOr (BitVec 64) :=
+      elemToCast.getN 0 (by simp [DialectSignature.sig, signature])
+    builtin.unrealized_conversion_cast.LLVMToriscv toCast
 
 @[simp_denote]
 def ctxtTransformToLLVM  (Γ : Ctxt LLVMPlusRiscV.Ty) :=
@@ -138,8 +133,7 @@ theorem outTy_map_signature_eq {s : Signature α} {f : α → β} :
 /- We tag the following definitions as `simp` and `simp_denote`
    so that `simp_peephole` and `simp` include them during simplification. -/
 attribute [simp, simp_denote] outTy_map_signature_eq
-
-attribute [simp, simp_denote] HVector.ubermapM
-attribute [simp, simp_denote] HVector.ubermap
+attribute [simp, simp_denote] HVector.mapM'
+attribute [simp, simp_denote] HVector.map'
 
 end LLVMRiscV
